Splitting off fresh_provenance from allocation functions.
Hoping this makes it easier to reuse the chunk without the fresh
provenance part for proofs.

src/coq/Handlers/MemoryModel.v
@@ -2863,12 +2863,17 @@ Module Type MemoryModelSpec (LP : LLVMParams) (MP : MemoryParams LP) (MMSP : Mem
              allocate_bytes_post_conditions m1 t init_bytes prov m2 ptr ptrs /\ ptr = ptr' /\ ptrs = ptrs'
          end.
 
+  Definition allocate_bytes_with_pr_spec_MemPropT
+    (t : dtyp) (init_bytes : list SByte) (prov : Provenance)
+    : MemPropT MemState addr
+    := '(ptr, ptrs) <- find_free_block (length init_bytes) prov;;
+       allocate_bytes_post_conditions_MemPropT t init_bytes prov ptr ptrs;;
+       ret ptr.
+
   Definition allocate_bytes_spec_MemPropT (t : dtyp) (init_bytes : list SByte)
     : MemPropT MemState addr
     := prov <- fresh_provenance;;
-       '(ptr, ptrs) <- find_free_block (length init_bytes) prov;;
-       allocate_bytes_post_conditions_MemPropT t init_bytes prov ptr ptrs;;
-       ret ptr.
+       allocate_bytes_with_pr_spec_MemPropT t init_bytes prov.
 
   (*** Allocating bytes in the heap *)
   Record malloc_bytes_post_conditions (m1 : MemState) (init_bytes : list SByte) (pr : Provenance) (m2 : MemState) (ptr : addr) (ptrs : list addr) : Prop :=
@@ -2915,12 +2920,16 @@ Module Type MemoryModelSpec (LP : LLVMParams) (MP : MemoryParams LP) (MMSP : Mem
              malloc_bytes_post_conditions m1 init_bytes prov m2 ptr ptrs /\ ptr = ptr' /\ ptrs = ptrs'
          end.
 
+  Definition malloc_bytes_with_pr_spec_MemPropT (init_bytes : list SByte) (prov : Provenance)
+    : MemPropT MemState addr
+    := '(ptr, ptrs) <- find_free_block (length init_bytes) prov;;
+       malloc_bytes_post_conditions_MemPropT init_bytes prov ptr ptrs;;
+       ret ptr.
+
   Definition malloc_bytes_spec_MemPropT (init_bytes : list SByte)
     : MemPropT MemState addr
     := prov <- fresh_provenance;;
-       '(ptr, ptrs) <- find_free_block (length init_bytes) prov;;
-       malloc_bytes_post_conditions_MemPropT init_bytes prov ptr ptrs;;
-       ret ptr.
+       malloc_bytes_with_pr_spec_MemPropT init_bytes prov.
 
   (*** Freeing heap allocations *)
   Record free_operation_invariants (m1 : MemState) (m2 : MemState) :=
@@ -4208,16 +4217,16 @@ Module Type MemoryModelExecPrimitives (LP : LLVMParams) (MP : MemoryParams LP).
       forall `{MemMonad ExtraState MemM (itree Eff)}, addr -> SByte -> MemM unit.
 
     (** Stack allocations *)
-    Parameter allocate_bytes :
-      forall `{MemMonad ExtraState MemM (itree Eff)}, dtyp -> list SByte -> MemM addr.
+    Parameter allocate_bytes_with_pr :
+      forall `{MemMonad ExtraState MemM (itree Eff)}, dtyp -> list SByte -> Provenance -> MemM addr.
 
     (** Frame stacks *)
     Parameter mempush : forall `{MemMonad ExtraState MemM (itree Eff)}, MemM unit.
     Parameter mempop : forall `{MemMonad ExtraState MemM (itree Eff)}, MemM unit.
 
     (** Heap operations *)
-    Parameter malloc_bytes :
-      forall `{MemMonad ExtraState MemM (itree Eff)}, list SByte -> MemM addr.
+    Parameter malloc_bytes_with_pr :
+      forall `{MemMonad ExtraState MemM (itree Eff)}, list SByte -> Provenance -> MemM addr.
 
     Parameter free :
       forall `{MemMonad ExtraState MemM (itree Eff)}, addr -> MemM unit.
@@ -4231,8 +4240,8 @@ Module Type MemoryModelExecPrimitives (LP : LLVMParams) (MP : MemoryParams LP).
     Parameter write_byte_correct :
       forall ptr byte pre, exec_correct pre (write_byte ptr byte) (write_byte_spec_MemPropT ptr byte).
 
-    Parameter allocate_bytes_correct :
-      forall dt init_bytes pre, exec_correct pre (allocate_bytes dt init_bytes) (allocate_bytes_spec_MemPropT dt init_bytes).
+    Parameter allocate_bytes_with_pr_correct :
+      forall dt init_bytes pr pre, exec_correct pre (allocate_bytes_with_pr dt init_bytes pr) (allocate_bytes_with_pr_spec_MemPropT dt init_bytes pr).
 
     (** Correctness of frame stack operations *)
     Parameter mempush_correct :
@@ -4241,9 +4250,9 @@ Module Type MemoryModelExecPrimitives (LP : LLVMParams) (MP : MemoryParams LP).
     Parameter mempop_correct :
       forall pre, exec_correct pre mempop mempop_spec_MemPropT.
 
-    Parameter malloc_bytes_correct :
-      forall init_bytes pre,
-        exec_correct pre (malloc_bytes init_bytes) (malloc_bytes_spec_MemPropT init_bytes).
+    Parameter malloc_bytes_with_pr_correct :
+      forall init_bytes pr pre,
+        exec_correct pre (malloc_bytes_with_pr init_bytes pr) (malloc_bytes_with_pr_spec_MemPropT init_bytes pr).
 
     Parameter free_correct :
       forall ptr pre,
@@ -4340,11 +4349,20 @@ Module Type MemoryModelExec (LP : LLVMParams) (MP : MemoryParams LP) (MMEP : Mem
       write_bytes ptr bytes.
 
     (** Allocating dtyps *)
+    Definition allocate_bytes `{MemMonad ExtraState MemM (itree Eff)} (dt : dtyp) (init_bytes : list SByte) : MemM addr :=
+      pr <- fresh_provenance;;
+      allocate_bytes_with_pr dt init_bytes pr.
+
     (* Need to make sure MemPropT has provenance and sids to generate the bytes. *)
     Definition allocate_dtyp `{MemMonad ExtraState MemM (itree Eff)} (dt : dtyp) : MemM addr :=
       sid <- fresh_sid;;
       bytes <- lift_OOM (generate_undef_bytes dt sid);;
       allocate_bytes dt bytes.
+
+    (** Malloc *)
+    Definition malloc_bytes `{MemMonad ExtraState MemM (itree Eff)} (init_bytes : list SByte) : MemM addr :=
+      pr <- fresh_provenance;;
+      malloc_bytes_with_pr init_bytes pr.
 
     (** Handle memcpy *)
     Definition memcpy `{MemMonad ExtraState MemM (itree Eff)} (src dst : addr) (len : Z) (align : N) (volatile : bool) : MemM unit :=
@@ -4625,6 +4643,19 @@ Module MemoryModelTheory (LP : LLVMParams) (MP : MemoryParams LP) (MMEP : Memory
       apply write_bytes_correct.
     Qed.
 
+    Lemma allocate_bytes_correct :
+      forall dt bytes pre,
+        exec_correct pre (allocate_bytes dt bytes) (allocate_bytes_spec_MemPropT dt bytes).
+    Proof.
+      intros dt pr pre.
+      apply exec_correct_bind.
+      apply exec_correct_fresh_provenance.
+      intros a ms_init ms_after_m st_init st_after_m RUN0.
+      apply allocate_bytes_with_pr_correct.
+    Qed.
+
+    Hint Resolve allocate_bytes_correct : EXEC_CORRECT.
+
     Lemma allocate_dtyp_correct :
       forall dt pre,
         exec_correct pre (allocate_dtyp dt) (allocate_dtyp_spec dt).
@@ -4693,6 +4724,17 @@ Module MemoryModelTheory (LP : LLVMParams) (MP : MemoryParams LP) (MMEP : Memory
       unfold handle_memcpy, handle_memcpy_prop.
       repeat (break_match; try apply exec_correct_raise_error).
       all: apply memcpy_correct.
+    Qed.
+
+    Lemma malloc_bytes_correct :
+      forall bytes pre,
+        exec_correct pre (malloc_bytes bytes) (malloc_bytes_spec_MemPropT bytes).
+    Proof.
+      intros bytes pre.
+      apply exec_correct_bind.
+      apply exec_correct_fresh_provenance.
+      intros a ms_init ms_after_m st_init st_after_m RUN0.
+      apply malloc_bytes_with_pr_correct.
     Qed.
 
     Hint Resolve malloc_bytes_correct : EXEC_CORRECT.
@@ -5032,13 +5074,13 @@ Module Type MemoryModelInfiniteSpec (LP : LLVMParamsBig) (MP : MemoryParams LP) 
   Import MP.BYTE_IMPL.
 
   Parameter find_free_block_can_always_succeed :
-    forall (ms : MemState) (len : nat) (pr : Provenance),
+    forall ms (len : nat) (pr : Provenance),
     exists ptr ptrs,
-      find_free_block len pr ms (ret (ms, (ptr, ptrs))).
+      ret (ptr, ptrs) {{ms}} ∈ {{ms}} find_free_block len pr.
 
   Parameter allocate_bytes_post_conditions_can_always_be_satisfied :
     forall (ms_init : MemState) dt bytes pr ptr ptrs
-      (FIND_FREE : find_free_block (length bytes) pr ms_init (ret (ms_init, (ptr, ptrs))))
+      (FIND_FREE : ret (ptr, ptrs) {{ms_init}} ∈ {{ms_init}} find_free_block (length bytes) pr)
       (BYTES_SIZE : sizeof_dtyp dt = N.of_nat (length bytes))
       (NON_VOID : dt <> DTYPE_Void),
     exists ms_final,
@@ -5075,7 +5117,7 @@ Module MemoryModelInfiniteSpecHelpers (LP : LLVMParamsBig) (MP : MemoryParams LP
       (BYTES_SIZE : sizeof_dtyp dt = N.of_nat (length bytes))
       (NON_VOID : dt <> DTYPE_Void),
     exists ms_final ptr,
-      allocate_bytes_spec_MemPropT dt bytes ms_init (ret (ms_final, ptr)).
+      ret ptr {{ms_init}} ∈ {{ms_final}} allocate_bytes_spec_MemPropT dt bytes.
   Proof.
     intros ms_init ms_fresh_pr dt bytes pr FRESH_PR BYTES_SIZE NON_VOID.
     unfold allocate_bytes_spec_MemPropT.
@@ -5149,7 +5191,7 @@ Module MemoryModelInfiniteSpecHelpers (LP : LLVMParamsBig) (MP : MemoryParams LP
       (FRESH_PR : (fresh_provenance ms_fresh_sid (ret (ms_fresh_pr, pr))))
       (NON_VOID : dt <> DTYPE_Void),
     exists ms_final ptr,
-      allocate_dtyp_spec dt ms_init (ret (ms_final, ptr)).
+      ret ptr {{ms_init}} ∈ {{ms_final}} allocate_dtyp_spec dt.
   Proof.
     intros ms_init ms_fresh_sid ms_fresh_pr dt pr sid FRESH_SID FRESH_PR NON_VOID.
 
